renamed: br -> wi
BitRange -> WordInterval

Primitive_Matchers/IpAddresses.thy
@@ -140,26 +140,26 @@ subsection{*IPv4 Addresses in IPTables Notation (how we parse it)*}
   text{*The @{typ "32 wordinterval"} can be translated back into a list of IP ranges.
         If a list of intervals is enough, we can use @{const br2l}.
         If we need it in @{typ ipt_ipv4range}, we can use this function.*}
-  definition br_2_cidr_ipt_ipv4range_list :: "32 wordinterval \<Rightarrow> ipt_ipv4range list" where
-    "br_2_cidr_ipt_ipv4range_list r = map (\<lambda> (base, len). Ip4AddrNetmask (dotdecimal_of_ipv4addr base) len) (ipv4range_split r)"
+  definition wi_2_cidr_ipt_ipv4range_list :: "32 wordinterval \<Rightarrow> ipt_ipv4range list" where
+    "wi_2_cidr_ipt_ipv4range_list r = map (\<lambda> (base, len). Ip4AddrNetmask (dotdecimal_of_ipv4addr base) len) (ipv4range_split r)"
 
-  lemma br_2_cidr_ipt_ipv4range_list: "(\<Union> ip \<in> set (br_2_cidr_ipt_ipv4range_list r). ipv4s_to_set ip) = wordinterval_to_set r"
+  lemma wi_2_cidr_ipt_ipv4range_list: "(\<Union> ip \<in> set (wi_2_cidr_ipt_ipv4range_list r). ipv4s_to_set ip) = wordinterval_to_set r"
     proof -
     have "\<And>a. ipv4s_to_set (case a of (base, x) \<Rightarrow> Ip4AddrNetmask (dotdecimal_of_ipv4addr base) x) = (case a of (x, xa) \<Rightarrow> ipv4range_set_from_bitmask x xa)"
       by(clarsimp simp add: ipv4addr_of_dotdecimal_dotdecimal_of_ipv4addr)
-    hence "(\<Union> ip \<in> set (br_2_cidr_ipt_ipv4range_list r). ipv4s_to_set ip) = \<Union>((\<lambda>(x, y). ipv4range_set_from_bitmask x y) ` set (ipv4range_split r))"
-      unfolding br_2_cidr_ipt_ipv4range_list_def by(simp)
+    hence "(\<Union> ip \<in> set (wi_2_cidr_ipt_ipv4range_list r). ipv4s_to_set ip) = \<Union>((\<lambda>(x, y). ipv4range_set_from_bitmask x y) ` set (ipv4range_split r))"
+      unfolding wi_2_cidr_ipt_ipv4range_list_def by(simp)
     thus ?thesis
     using ipv4range_split_bitmask by presburger
   qed
 
   text{*For example, this allows the following transformation*}
   definition ipt_ipv4range_compress :: "ipt_ipv4range negation_type list \<Rightarrow> ipt_ipv4range list" where
-    "ipt_ipv4range_compress = br_2_cidr_ipt_ipv4range_list \<circ> ipt_ipv4range_negation_type_to_br_intersect"
+    "ipt_ipv4range_compress = wi_2_cidr_ipt_ipv4range_list \<circ> ipt_ipv4range_negation_type_to_br_intersect"
 
   lemma ipt_ipv4range_compress: "(\<Union> ip \<in> set (ipt_ipv4range_compress l). ipv4s_to_set ip) =
       (\<Inter> ip \<in> set (getPos l). ipv4s_to_set ip) - (\<Union> ip \<in> set (getNeg l). ipv4s_to_set ip)"
-    by (metis br_2_cidr_ipt_ipv4range_list comp_apply ipt_ipv4range_compress_def ipt_ipv4range_negation_type_to_br_intersect)
+    by (metis wi_2_cidr_ipt_ipv4range_list comp_apply ipt_ipv4range_compress_def ipt_ipv4range_negation_type_to_br_intersect)
       
 
 end
